\documentclass{article}
\usepackage{amsmath}

\begin{document}

\begin{gather}
    \frac{\frac{-3\frac{21}{80}}{\frac{1}{8}}}{\left(5\frac{1}{2} - 1\right) \cdot \frac{2}{3}} + 3\frac{11}{30} - 2\frac{2}{3} = -8 \\
    \frac{-45\frac{5}{12} - \frac{1}{3}}{\frac{3}{5}} + \frac{\left(3\frac{1}{20} - \frac{4}{5}\right) \cdot 1}{9} = -76 \\
    \frac{-\frac{9}{14}}{2\frac{13}{70} - \frac{9}{10}} + \frac{\frac{9}{16} \cdot \frac{2}{9}}{\frac{11}{20} - \frac{3}{10}} = 0 \\
    \frac{\frac{-636\frac{4}{81}}{8}}{\left(2\frac{1}{3} - \frac{5}{9}\right) \cdot \frac{1}{2}} + 4\frac{4}{9} - 4 = -89 \\
    \frac{2\frac{17}{45} - \frac{3}{5}}{\frac{2}{3}} + \left(4\frac{7}{12} - 1\frac{1}{4}\right) \cdot \frac{1\frac{2}{5}}{3\frac{1}{2}} = 4 \\
    \frac{16\frac{4}{15} - \frac{1}{5}}{\frac{1}{3}} + \frac{2}{5} \cdot \frac{1\frac{5}{9}}{2\frac{5}{18} - 1\frac{1}{2}} = 49 \\
    196 \cdot \frac{1}{7} + \frac{\frac{5}{6} - \frac{2}{3}}{\frac{\frac{73}{90} - \frac{7}{9}}{\frac{1}{5}}} = 29 \\
    \frac{81\frac{5}{24} - \frac{3}{8}}{\frac{2\frac{1}{12}}{1\frac{1}{4}}} + \left(1\frac{3}{10} - 1\right) \cdot 1\frac{2}{3} = 49 \\
    \frac{\frac{-38\frac{5}{8}}{2\frac{3}{4} - \frac{1}{2}}}{1\frac{2}{3} \cdot \frac{1}{3}} + 5\frac{2}{5} - 4\frac{1}{2} = -30 \\
    \frac{17\frac{7}{8} - 1}{5} + \frac{\frac{5}{28} \cdot \left(8\frac{3}{5} - 1\frac{3}{5}\right)}{2} = 4 \\
    -95\frac{2}{5} - \frac{1}{2} - \frac{3}{5} + \frac{3\frac{1}{2}}{28 \cdot \frac{\frac{1}{8}}{\frac{1}{2}}} = -96 \\
    \frac{28\frac{1}{5} \cdot 1}{\frac{1}{3}} + \frac{7\frac{6}{25} - 7}{1\frac{9}{40} - \frac{5}{8}} = 85 \\
    \frac{-74\frac{1}{5}}{1\frac{2}{5}} + \frac{3\frac{5}{6} - \frac{5}{6}}{1\frac{1}{2} \cdot \left(1\frac{3}{8} - \frac{3}{8}\right)} = -51 \\
    \left(-46 - 2\right) \cdot \frac{2\frac{5}{8}}{2\frac{1}{3}} + \frac{8\frac{2}{3} - 7}{1\frac{2}{3}} = -53 \\
    -64\frac{1}{2} - \left(1\frac{3}{10} - \frac{4}{5}\right) + \frac{\frac{1}{3} \cdot \frac{\frac{1}{4}}{\frac{1}{6}}}{\frac{1}{4}} = -63
\end{gather}

\begin{gather}
    \frac{58\frac{1}{20} \cdot \frac{\frac{28}{45}}{1\frac{2}{5}}}{9\frac{3}{5} - 9} + 1\frac{3}{5} - \frac{3}{5} = 44 \\
    \frac{-49 - 9}{3\frac{3}{4} \cdot 1\frac{1}{3}} + \frac{\frac{24}{25}}{3\frac{1}{10} - 1\frac{1}{2}} = -11 \\
    \frac{165\frac{3}{20}}{2\frac{1}{4} \cdot \frac{\frac{8}{9}}{\frac{8}{9}}} + 8\frac{3}{5} - \left(8\frac{1}{6} - \frac{1}{6}\right) = 74 \\
    60\frac{3}{4} - 1 + \frac{3\frac{11}{48} - 2\frac{2}{3}}{\frac{1\frac{1}{8}}{3\frac{1}{2}} \cdot \frac{7}{9}} = 62 \\
    \frac{-185\frac{5}{8}}{4\frac{3}{4} - \frac{1}{4}} \cdot 2 + \frac{1\frac{1}{2}}{1\frac{1}{3} - \frac{1}{3}} = -81 \\
    \frac{-25\frac{2}{5}}{\frac{1}{2}} + \left(2\frac{1}{45} - \frac{2}{9}\right) \cdot \frac{\frac{6}{7}}{1\frac{6}{7} - 1} = -49 \\
    63\frac{2}{9} + \frac{5\frac{4}{9} \cdot \frac{1\frac{3}{5}}{1\frac{3}{5}}}{8\frac{7}{9} - \frac{7}{9} - 1} = 64 \\
    \frac{39\frac{5}{9} \cdot \frac{2}{5}}{2\frac{3}{5} - 1} + \frac{\frac{1}{81}}{1\frac{4}{9} - 1\frac{1}{3}} = 10 \\
    \frac{189\frac{3}{4}}{4\frac{3}{4} - 2\frac{1}{2}} + \frac{\frac{3}{4}}{\frac{3}{4}} \cdot \left(2\frac{1}{15} - 1\frac{2}{5}\right) = 85 \\
    \frac{\frac{-55\frac{13}{14}}{\frac{1}{7}}}{10\frac{3}{8} - 1\frac{1}{8} - \frac{1}{4}} + \frac{2}{3} \cdot \frac{3}{4} = -43 \\
    \frac{-36\frac{1}{14}}{1\frac{1}{4}} \cdot \left(1\frac{1}{8} - \frac{1}{8}\right) + \frac{3\frac{2}{7} - 1}{2\frac{2}{3}} = -28 \\
    \left(12\frac{3}{25} - 1\frac{4}{5}\right) \cdot \frac{5}{6} + \frac{2\frac{1}{5} - 1}{\frac{\frac{12}{35}}{\frac{2}{5}}} = 10 \\
    \frac{-27\frac{9}{14}}{\frac{1\frac{5}{7} - \left(3\frac{1}{2} - 2\right)}{\frac{9}{10}} \cdot 1\frac{4}{5}} + \frac{1}{2} = -64 \\
    \frac{-2\frac{3}{10}}{\frac{1\frac{2}{3}}{4\frac{2}{3} - 3}} + \left(1\frac{3}{10} - 1\right) \cdot 1 = -2 \\
    \frac{-750\frac{2}{5}}{8} + \frac{\frac{14}{15}}{2\frac{11}{40} - 1\frac{2}{5}} \cdot \left(1\frac{5}{28} - \frac{3}{7}\right) = -93
\end{gather}

\begin{gather}
    66\frac{1}{6} - 6 + \frac{\frac{5}{42}}{\frac{1}{35} \cdot \frac{4\frac{3}{8}}{1\frac{47}{72} - \frac{7}{9}}} = 61 \\
    -286\frac{3}{10} \cdot \frac{2}{7} + \frac{\frac{\frac{14}{15}}{1\frac{2}{5}}}{3\frac{1}{2} - 1\frac{1}{6} - 1\frac{1}{2}} = -81 \\
    \frac{48\frac{7}{16}}{\frac{\frac{173}{288} - \frac{4}{9}}{\frac{1}{4}}} + 2 \cdot \left(2\frac{3}{4} - 1\right) = 81 \\
    \frac{-792 - 4\frac{1}{2}}{\frac{46\frac{2}{7}}{4\frac{1}{7} - 3} \cdot \frac{2}{9}} + 1\frac{1}{2} = -87 \\
    \frac{124\frac{1}{2}}{3 \cdot \frac{1}{2}} + \frac{6 - 1}{1\frac{3}{4} - \frac{1}{2}} = 87 \\
    \frac{-385\frac{1}{5}}{4\frac{9}{14} - \left(1\frac{1}{7} - 1\right)} + \frac{\frac{9}{10}}{1\frac{1}{2}} \cdot 1 = -85 \\
    \frac{\frac{20\frac{5}{21}}{1\frac{8}{21} - \frac{5}{7}}}{1\frac{1}{2} \cdot \frac{1}{3}} + \frac{32}{63} - \frac{2}{9} = 61 \\
    \frac{1\frac{1}{2}}{\frac{1\frac{1}{15}}{1\frac{1}{3}}} + \left(8\frac{1}{4} - 8\right) \cdot \left(\frac{4}{5} - \frac{3}{10}\right) = 2 \\
    \frac{-9\frac{7}{36} - 1\frac{1}{2}}{\frac{7}{12} - \frac{1}{3}} + \frac{\frac{7}{27} \cdot \frac{3}{5}}{\frac{1}{5}} = -42 \\
    \frac{62\frac{14}{15} \cdot 1}{3\frac{2}{15} - 2\frac{1}{3}} + \frac{\frac{41}{54} - \frac{1}{2}}{\frac{7}{9}} = 79 \\
    -115\frac{5}{6} \cdot \frac{\frac{2}{15}}{\frac{2}{9}} + \frac{2\frac{3}{10} - 2\frac{1}{4}}{\frac{7}{20} - \frac{1}{4}} = -69 \\
    \left(111\frac{1}{35} - \frac{6}{7}\right) \cdot \frac{\frac{7}{16}}{\frac{1}{2}} + \frac{\frac{3}{5}}{2\frac{1}{4} - 1\frac{1}{4}} = 97 \\
    81 - \left(9 - 3\right) + \frac{20\frac{1}{4}}{3\frac{3}{8} \cdot \frac{\frac{7}{15}}{\frac{7}{10}}} = 84 \\
    -39\frac{11}{21} \cdot \left(2\frac{4}{5} - 1\right) + \frac{\frac{\frac{3}{112}}{\frac{1}{2}}}{1\frac{7}{40} - \frac{4}{5}} = -71 \\
    \frac{160}{4 - 2} + \frac{1}{7 \cdot \left(1\frac{1}{7} - 1\right)} = 81
\end{gather}

\end{document}
